unwrapped PCM from scratch: lseq a n & lseq perm n
focus now on Steel.Array9
add Steel.Array7,
traduction from wrapped PCM to unwrapped PCM

src/Steel.Array7.fsti
@@ -28,11 +28,21 @@ let comp_prop (#a: Type) (x y: a & perm)
   = fst x == fst y /\ (sum_perm (snd x) (snd y)).v <=. one
 
 let composable' (#a: Type) : symrel (seq (a & perm))
-  = fun (arr1 arr2: seq (a & perm))  ->
+  = fun (arr1 arr2: seq (a & perm)) ->
   length arr1 == length arr2 /\
   (forall (i:nat{i < length arr1}).
     comp_prop (index arr1 i) (index arr2 i)
   )
+
+let content (a: Type u#1) : Type u#1
+  = x:(seq a & seq perm){length (fst x) == length (snd x)}
+let array2 (a: Type u#1) : Type u#1 = option (content a)
+
+let composable2' (#a: Type) : symrel (content a)
+  = fun (arr1 arr2: content a) ->
+  let arr1 = zip (fst arr1) (snd arr1) in
+  let arr2 = zip (fst arr2) (snd arr2) in
+  composable' arr1 arr2
 
 let composable (#a: Type) : symrel (array a)
   = fun (arr1 arr2: array a)
@@ -40,6 +50,22 @@ let composable (#a: Type) : symrel (array a)
   | None, _
   | _,  None -> True
   | Some c1, Some c2 -> composable' c1 c2
+
+let composable2 (#a: Type) : symrel (array2 a)
+  = fun (arr1 arr2: array2 a)
+  -> match arr1, arr2 with
+  | None, _
+  | _, None -> True
+  | Some c1, Some c2 -> composable2' c1 c2
+
+let composable2'_to_len_eq (#a: Type) (arr1 arr2: content a)
+  : Lemma
+  (requires composable2' arr1 arr2)
+  (ensures length (fst arr1) == length (fst arr2))
+  =
+  zip_len (fst arr1) (snd arr1);
+  zip_len (fst arr2) (snd arr2);
+  ()
 
 let f (#a: Type) : a & perm -> a & perm -> a & perm =
   fun x y -> (fst x, (sum_perm (snd x) (snd y)))
@@ -51,6 +77,22 @@ let op' (#a: Type)
   map_seq2_len f s1 s2;
   map_seq2 f s1 s2
 
+let op2' (#a: Type)
+  (s1: content a) (s2: content a{length (fst s1) == length (fst s2)})
+  : (r: content a{length (fst r) == length (fst s1)})
+  =
+  assert (length (fst s1) == length (snd s1));
+  assert (length (fst s2) == length (snd s2));
+  assert (length (fst s1) == length (fst s2));
+  zip_len (fst s1) (snd s1);
+  zip_len (fst s2) (snd s2);
+  let s1 : seq (a & perm) = zip (fst s1) (snd s1) in
+  let s2 : seq (a & perm) = zip (fst s2) (snd s2) in
+  assert (length s1 == length s2);
+  let r = op' s1 s2 in
+  unzip_len r;
+  unzip r
+
 let op (#a: Type)
   (arr1: array a) (arr2: array a {composable arr1 arr2})
   : array a
@@ -59,9 +101,25 @@ let op (#a: Type)
   | f, None -> f
   | Some s1, Some s2 -> Some (op' s1 s2)
 
+let op2 (#a: Type)
+  (arr1: array2 a) (arr2: array2 a {composable2 arr1 arr2})
+  = match arr1, arr2 with
+  | None, f
+  | f, None -> f
+  | Some s1, Some s2 ->
+      assert (composable2' s1 s2);
+      composable2'_to_len_eq s1 s2;
+      Some (op2' s1 s2)
+
 let pcm_array' (#a: Type) : pcm' (array a) = {
   composable = composable;
   op = op;
+  one = None;
+}
+
+let pcm_array2' (#a: Type) : pcm' (array2 a) = {
+  composable = composable2;
+  op = op2;
   one = None;
 }
 
@@ -75,6 +133,19 @@ let lem_commutative (#a: Type)
     assert (composable arr1 arr2);
     assert (length s1 == length s2);
     map_seq2_comm f s1 s2
+
+let lem_commutative2 (#a: Type)
+  (arr1: array2 a) (arr2: array2 a {composable2 arr1 arr2})
+  : Lemma (op2 arr1 arr2 == op2 arr2 arr1)
+  = match arr1, arr2 with
+  | None, _
+  | _, None -> ()
+  | Some s1, Some s2 ->
+      zip_len (fst s1) (snd s1);
+      zip_len (fst s2) (snd s2);
+      let s1 : seq (a & perm) = zip (fst s1) (snd s1) in
+      let s2 : seq (a & perm) = zip (fst s2) (snd s2) in
+      lem_commutative (Some s1) (Some s2)
 
 let lem_assoc_l_eq (#a: Type)
   (arr1 arr2 arr3: array a)
@@ -220,6 +291,150 @@ let lem_assoc (#a: Type)
   ()
   end
 
+let composable_to_composable2 (#a: Type) (arr1 arr2: array a)
+  : Lemma
+  (requires
+    Some? arr1 /\
+    Some? arr2 /\
+    composable arr1 arr2)
+  (ensures (
+    let arr1' = unzip (Some?.v arr1) in
+    let arr2' = unzip (Some?.v arr2) in
+    unzip_len (Some?.v arr1);
+    unzip_len (Some?.v arr2);
+    composable2 (Some arr1') (Some arr2')))
+  = admit ()
+
+let composable_op_to_composable2_op (#a: Type)
+  (arr1 arr2 arr3: array a)
+  : Lemma
+  (requires
+    Some? arr1 /\
+    Some? arr2 /\
+    Some? arr3 /\
+    composable arr2 arr3 /\
+    composable arr1 (op arr2 arr3))
+  (ensures (
+    let arr1' = unzip (Some?.v arr1) in
+    let arr2' = unzip (Some?.v arr2) in
+    let arr3' = unzip (Some?.v arr3) in
+    unzip_len (Some?.v arr1);
+    unzip_len (Some?.v arr2);
+    unzip_len (Some?.v arr3);
+    composable2 (Some arr2') (Some arr3') /\
+    composable2 (Some arr1') (op2 (Some arr2') (Some arr3'))))
+  = admit ()
+
+let composable2_to_composable (#a: Type) (arr1 arr2: array2 a)
+  : Lemma
+  (requires
+    Some? arr1 /\
+    Some? arr2 /\
+    composable2 arr1 arr2)
+  (ensures (
+    let arr1' = zip (fst (Some?.v arr1)) (snd (Some?.v arr1)) in
+    let arr2' = zip (fst (Some?.v arr2)) (snd (Some?.v arr2)) in
+    zip_len (fst (Some?.v arr1)) (snd (Some?.v arr1));
+    zip_len (fst (Some?.v arr2)) (snd (Some?.v arr2));
+    composable (Some arr1') (Some arr2')))
+  = ()
+
+let composable2_op_to_composable_op (#a: Type)
+  (arr1 arr2 arr3: array2 a)
+  : Lemma
+  (requires
+    Some? arr1 /\
+    Some? arr2 /\
+    Some? arr3 /\
+    composable2 arr2 arr3 /\
+    composable2 arr1 (op2 arr2 arr3))
+  (ensures (
+    let arr1' = zip (fst (Some?.v arr1)) (snd (Some?.v arr1)) in
+    let arr2' = zip (fst (Some?.v arr2)) (snd (Some?.v arr2)) in
+    let arr3' = zip (fst (Some?.v arr3)) (snd (Some?.v arr3)) in
+    zip_len (fst (Some?.v arr1)) (snd (Some?.v arr1));
+    zip_len (fst (Some?.v arr2)) (snd (Some?.v arr2));
+    zip_len (fst (Some?.v arr3)) (snd (Some?.v arr3));
+    composable (Some arr2') (Some arr3') /\
+    composable (Some arr1') (op (Some arr2') (Some arr3'))
+  ))
+  = admit ()
+
+let op_eq_to_op2_eq (#a: Type)
+  (arr1 arr2 arr3: array a)
+  : Lemma
+  (requires
+    Some? arr1 /\
+    Some? arr2 /\
+    composable arr1 arr2 /\
+    arr3 == op arr1 arr2
+  )
+  (ensures (
+    unzip_len (Some?.v arr1);
+    unzip_len (Some?.v arr2);
+    unzip_len (Some?.v arr3);
+    let arr1' = Some (unzip (Some?.v arr1)) in
+    let arr2' = Some (unzip (Some?.v arr2)) in
+    let arr3' = Some (unzip (Some?.v arr3)) in
+    composable_to_composable2 arr1 arr2;
+    assert (composable2 arr1' arr2');
+    admit ();
+    //Classical.forall_intro (zip_unzip_id #(a & perm));
+    arr3' == op2 arr1' arr2'
+  ))
+  = admit ()
+
+let lem_assoc2 (#a: Type)
+  (arr1 arr2 arr3: array2 a)
+  : Lemma
+  (requires
+    composable2 arr2 arr3 /\
+    composable2 arr1 (op2 arr2 arr3)
+  )
+  (ensures
+    composable2 arr1 arr2 /\
+    composable2 (op2 arr1 arr2) arr3 /\
+    op2 arr1 (op2 arr2 arr3) == op2 (op2 arr1 arr2) arr3
+  )
+  =
+  if None? arr1 then () else
+  if None? arr2 then () else
+  if None? arr3 then () else begin
+    let s1 = Some?.v arr1 in
+    let s2 = Some?.v arr2 in
+    let s3 = Some?.v arr3 in
+    zip_len (fst s1) (snd s1);
+    zip_len (fst s2) (snd s2);
+    zip_len (fst s3) (snd s3);
+    let s1 : seq (a & perm) = zip (fst s1) (snd s1) in
+    let s2 : seq (a & perm) = zip (fst s2) (snd s2) in
+    let s3 : seq (a & perm) = zip (fst s3) (snd s3) in
+    composable2_to_composable arr2 arr3;
+    composable2_op_to_composable_op arr1 arr2 arr3;
+    lem_assoc (Some s1) (Some s2) (Some s3);
+    assert (
+      composable (Some s1) (Some s2) /\
+      composable (op (Some s1) (Some s2)) (Some s3) /\
+      op (Some s1) (op (Some s2) (Some s3))
+      == op (op (Some s1) (Some s2)) (Some s3)
+    );
+    assert (
+      composable (Some s1) (Some s2) /\
+      composable (Some s3) (op (Some s1) (Some s2))
+    );
+    composable_op_to_composable2_op (Some s3) (Some s1) (Some s2);
+    Classical.forall_intro_2 (unzip_zip_id #a #perm);
+    op_eq_to_op2_eq (Some s1) (Some s2) (op (Some s1) (Some s2));
+    op_eq_to_op2_eq
+      (Some s1) (op (Some s2) (Some s3))
+      (op (Some s1) (op (Some s2) (Some s3)));
+    admit ();
+    op_eq_to_op2_eq
+      (op (Some s1) (Some s2)) (Some s3)
+      (op (op (Some s2) (Some s3)) (Some s3));
+    ()
+  end
+
 let lem_assoc_l (#a: Type)
   (arr1 arr2: array a) (arr3: array a{
     composable arr2 arr3 /\ composable arr1 (op arr2 arr3)
@@ -231,6 +446,18 @@ let lem_assoc_l (#a: Type)
   )
   =
   lem_assoc arr1 arr2 arr3
+
+let lem_assoc_l2 (#a: Type)
+  (arr1 arr2: array2 a) (arr3: array2 a{
+    composable2 arr2 arr3 /\ composable2 arr1 (op2 arr2 arr3)
+  })
+  : Lemma (
+    composable2 arr1 arr2 /\
+    composable2 (op2 arr1 arr2) arr3 /\
+    op2 arr1 (op2 arr2 arr3) == op2 (op2 arr1 arr2) arr3
+  )
+  =
+  lem_assoc2 arr1 arr2 arr3
 
 let lem_assoc_r (#a: Type)
   (arr1 arr2: array a) (arr3: array a{
@@ -248,6 +475,22 @@ let lem_assoc_r (#a: Type)
   lem_commutative arr1 (op arr2 arr3);
   lem_commutative arr3 (op arr1 arr2)
 
+let lem_assoc_r2 (#a: Type)
+  (arr1 arr2: array2 a) (arr3: array2 a{
+    composable2 arr1 arr2 /\ composable2 (op2 arr1 arr2) arr3
+  })
+  : Lemma (
+    composable2 arr2 arr3 /\
+    composable2 arr1 (op2 arr2 arr3) /\
+    op2 arr1 (op2 arr2 arr3) == op2 (op2 arr1 arr2) arr3
+  )
+  =
+  lem_commutative2 arr1 arr2;
+  lem_assoc2 arr3 arr2 arr1;
+  lem_commutative2 arr2 arr3;
+  lem_commutative2 arr1 (op2 arr2 arr3);
+  lem_commutative2 arr3 (op2 arr1 arr2)
+
 let pcm_array (#a: Type) : pcm (array a) = {
   p = pcm_array';
   comm = lem_commutative;
@@ -257,18 +500,38 @@ let pcm_array (#a: Type) : pcm (array a) = {
   refine = (fun _ -> True);
 }
 
+let pcm_array2 (#a: Type) : pcm (array2 a) = {
+  p = pcm_array2';
+  comm = lem_commutative2;
+  assoc = lem_assoc_l2;
+  assoc_r = lem_assoc_r2;
+  is_unit = (fun _ -> ());
+  refine = (fun _ -> True);
+}
+
 //val array_ref (a: Type u#0) : Type u#0
 let array_ref (a: Type u#1) : Type u#0
   = Mem.ref (array a) pcm_array
 
+let array_ref2 (a: Type u#1) : Type u#0
+  = Mem.ref (array2 a) pcm_array2
+
 let null #a = Mem.null #(array a) #pcm_array
+let null2 #a = Mem.null #(array2 a) #pcm_array2
+
 let is_null #a r = Mem.is_null #(array a) #pcm_array r
+let is_null2 #a r = Mem.is_null #(array2 a) #pcm_array2 r
 
 let perm_ok_elem p : prop = (p.v <=. one == true) /\ True
 
 let perm_ok #a (s: seq (a & perm)) : prop
   =
   forall i. ((snd (index s i)).v <=. one == true)
+
+
+let perm_ok3 (#a: Type) (#n: nat) (s: lseq a n & lseq perm n) : prop
+  =
+  forall i. ((index (snd s) i).v <=. one == true)
 
 let apply (#a: Type u#1) (s: seq (a & perm)) (p: perm)
   : (r:seq (a & perm){length r == length s})
@@ -336,18 +599,45 @@ let abcd_acbd (a b c d:Mem.slprop)
     ((a `star` c) `star` (b `star` d));
    }
 
-// stuck: need to separate perm from content
+let composable_to_fst_unzip_eq (#a: Type u#a)
+  (s1 s2: seq (a & perm))
+  : Lemma
+  (requires composable' s1 s2)
+  (ensures fst (unzip s1) == fst (unzip s2))
+  =
+  unzip_len s1;
+  unzip_len s2;
+  Classical.forall_intro (unzip_index s1);
+  Classical.forall_intro (unzip_index s2);
+  Seq.lemma_eq_elim (fst (unzip s1)) (fst (unzip s2))
+
+let op_to_fst_unzip_eq (#a: Type u#a)
+  (s1 s2 s3: seq (a & perm))
+  : Lemma
+  (requires
+    composable' s1 s2 /\
+    s3 == op' s1 s2)
+  (ensures
+    fst (unzip s1) == fst (unzip s3))
+  =
+  unzip_len s1;
+  unzip_len s2;
+  unzip_len s3;
+  Classical.forall_intro (unzip_index s1);
+  Classical.forall_intro (unzip_index s2);
+  Classical.forall_intro (unzip_index s3);
+  Classical.forall_intro (map_seq2_index f s1 s2);
+  Seq.lemma_eq_elim (fst (unzip s1)) (fst (unzip s3))
+
 let pts_to_ref_injective
   (#a: Type u#1)
   (r: array_ref a)
-  //(p0 p1:perm)
   (v0 v1: seq (a & perm))
   (m:Mem.mem)
   : Lemma
     (requires
       Mem.interp (pts_to_sl r v0 `Mem.star` pts_to_sl r v1) m)
     (ensures
-      //fst (unzip v0) `Seq.equal` fst (unzip v1)
       fst (unzip v0) == fst (unzip v1)
     )
   = let open Steel.Memory in
@@ -362,30 +652,7 @@ let pts_to_ref_injective
                             (Some v1)
                             m;
     assert (composable' v0 v1);
-    assert  (forall (i:nat{i < length v1}).
-      comp_prop (index v0 i) (index v1 i)
-    );
-    assert (length v0 == length v1);
-    assert  (forall (i:nat{i < length v1}).
-      (let x = index v0 i in
-      let y = index v1 i in
-      fst x == fst y /\ (sum_perm (snd x) (snd y)).v <=. one
-      )
-    );
-    let s0 = fst (unzip v0) in
-    let s1 = fst (unzip v1) in
-    unzip_len v0;
-    unzip_len v1;
-    assert (forall (i:nat{i < length v1}).
-      fst (index v0 i) == fst (index v1 i)
-    );
-    Classical.forall_intro (unzip_index v0);
-    Classical.forall_intro (unzip_index v1);
-    assert (forall (i:nat{i < length v1}).
-      index s0 i == index s1 i
-    );
-    Seq.lemma_eq_elim s0 s1;
-    ()
+    composable_to_fst_unzip_eq v0 v1
 
 let pts_to_not_null (#a:Type u#1)
                     (r:array_ref a)
@@ -393,22 +660,106 @@ let pts_to_not_null (#a:Type u#1)
                     (m:Mem.mem)
   : Lemma (requires Mem.interp (pts_to_sl r v) m)
           (ensures r =!= null)
-  = Mem.affine_star (hp_of (pts_to_raw r v)) (Mem.pure (perm_ok v)) m;
+  = Mem.affine_star
+      (hp_of (pts_to_raw r v))
+      (Mem.pure (perm_ok v)) m;
     Mem.pts_to_not_null r (Some v) m
 
-[@@ expect_failure]
-let pts_to_witinv (#a:Type) (r:array_ref a)
-  : Lemma (Mem.is_witness_invariant (pts_to_sl r)) =
-  let aux (x y: erased (seq (a & perm))) (m:Mem.mem)
-    : Lemma
-    (requires (
-      Mem.interp (pts_to_sl r x) m /\
-      Mem.interp (pts_to_sl r y) m))
-    (ensures (fst (unzip x) `Seq.equal` fst (unzip y)))
-    =
-    Mem.pts_to_join r (Some (reveal x)) (Some (reveal y)) m;
-    admit ();
-    //Seq.lemma_eq_elim (fst (unzip (reveal x))) (fst (unzip (reveal y)))
-    ()
-  in
-  Classical.forall_intro_3 (fun x y -> Classical.move_requires (aux x y))
+let aux' (#a: Type u#1)
+  (x y f1 f2 z: array a)
+  : Lemma
+  (requires
+    Some? x /\
+    Some? y /\
+    composable x f1 /\
+    op f1 x == z /\
+    composable y f2 /\
+    op f2 y == z
+  )
+  (ensures fst (unzip (Some?.v x)) == fst (unzip (Some?.v y)))
+  =
+  assert (Some? z);
+  match (Some? f1, Some? f2) with
+  | false, false -> ()
+  | true, false ->
+    assert (op f2 y == y);
+    assert (y == z);
+    composable_to_fst_unzip_eq (Some?.v x) (Some?.v f1);
+    op_to_fst_unzip_eq (Some?.v f1) (Some?.v x) (Some?.v z)
+  | false, true ->
+    assert (op f1 x == x);
+    assert (x == z);
+    composable_to_fst_unzip_eq (Some?.v y) (Some?.v f2);
+    op_to_fst_unzip_eq (Some?.v f2) (Some?.v y) (Some?.v z)
+  | true, true ->
+    composable_to_fst_unzip_eq (Some?.v x) (Some?.v f1);
+    composable_to_fst_unzip_eq (Some?.v y) (Some?.v f2);
+    op_to_fst_unzip_eq (Some?.v f1) (Some?.v x) (Some?.v z);
+    op_to_fst_unzip_eq (Some?.v f2) (Some?.v y) (Some?.v z)
+
+//#push-options "--z3rlimit 300 --query_stats"
+let aux (#a: Type u#1)
+  (r: array_ref a)
+  (x y: erased (seq (a & perm))) (m:Mem.mem)
+  : Lemma
+  (requires (
+    Mem.interp (pts_to_sl r x) m /\
+    Mem.interp (pts_to_sl r y) m /\
+    snd (unzip x) == snd (unzip y)
+  ))
+  (ensures (fst (unzip x) == fst (unzip y)))
+  =
+  Mem.pts_to_join r (Some (reveal x)) (Some (reveal y)) m;
+  assert (joinable pcm_array (Some (reveal x)) (Some (reveal y)));
+  assert (exists z.
+    compatible pcm_array (Some (reveal x)) z /\
+    compatible pcm_array (Some (reveal y)) z
+  );
+  assert (
+    let x' = Some (reveal x) in
+    let y' = Some (reveal y) in
+    exists z.
+    (exists (frame: array a).
+      composable x' frame /\
+      op frame x' == z) /\
+    (exists (frame: array a).
+      composable y' frame /\
+      op frame y' == z)
+  );
+  assert (
+    let x' = Some (reveal x) in
+    let y' = Some (reveal y) in
+    exists (z f1 f2: array a).
+      composable x' f1 /\
+      op f1 x' == z /\
+      composable y' f2 /\
+      op f2 y' == z /\
+      Some? z
+  );
+  Classical.forall_intro_3 (
+    Classical.move_requires_3 (
+        aux' (Some (reveal x)) (Some (reveal y))
+    )
+  );
+  ()
+
+// 1) better definition
+// 2) a pts_to wrapper? an unwrapped PCM based on the wrapped one?
+// seems relatively reasonable so far...
+let pts_to_witinv_aux (#a:Type) (r:array_ref a) (s2: seq perm)
+  : Lemma (
+  Mem.is_witness_invariant
+  (fun (s1: seq a{length s1 == length s2}) ->
+  pts_to_sl r (zip s1 s2)))
+  =
+  Classical.forall_intro_3 (
+    fun (x y: (s1:seq a{length s1 == length s2})) ->
+    (
+    zip_len x s2;
+    zip_len y s2;
+    Classical.forall_intro (zip_index x s2);
+    Classical.forall_intro (zip_index y s2);
+    assume (snd (unzip (zip x s2)) == snd (unzip (zip y s2)));
+    Classical.move_requires (aux r (zip x s2) (zip y s2))
+    )
+  )
