src/Steel.Array9.fsti
@@ -1,0 +1,494 @@
+module Steel.Array9
+
+open FStar.Ghost
+open Steel.Effect.Atomic
+open Steel.Effect
+open FStar.Real
+open FStar.PCM
+open Steel.FractionalPermission
+module RP = Steel.PCMReference
+module Mem = Steel.Memory
+
+#set-options "--ide_id_info_off"
+
+open FStar.Seq
+open Seq.Aux
+
+(**
+First step : seq (a & perm) pcm
+Second step : slprop on top of it
+Third step : vprop on top of it, introducing idx1/idx2
+**)
+
+(** First step **)
+
+let content (a: Type u#1) (#n: nat): Type u#1 = lseq a n & lseq perm n
+
+let array (a: Type u#1) (#n: nat): Type u#1 = option (content a #n)
+
+let comp_prop (#a: Type) (v1 v2: a) (p1 p2: perm)
+  = v1 == v2 /\ (sum_perm p1 p2).v <=. one
+
+let composable' (#a: Type) (#n: nat): symrel (content a #n)
+  = fun (arr1 arr2: content a #n) ->
+  (forall (i:nat{i < n}).
+    comp_prop
+      (index (fst arr1) i) (index (fst arr2) i)
+      (index (snd arr1) i) (index (snd arr2) i)
+  )
+
+let composable (#a: Type) (#n: nat): symrel (array a)
+  = fun (arr1 arr2: array a)
+  -> match arr1, arr2 with
+  | None, _
+  | _,  None -> True
+  | Some c1, Some c2 -> composable' #a #n c1 c2
+
+let f1 (#a: Type) : a -> a -> a
+  = fun x y -> x
+let f2 : perm -> perm -> perm
+  = fun x y -> sum_perm x y
+
+let f (#a: Type) : a & perm -> a & perm -> a & perm =
+  fun x y -> f1 (fst x) (fst y), f2 (snd x) (snd y)
+
+let op' (#a: Type) (#n: nat)
+  (s1: content a #n) (s2: content a #n)
+  : content a #n
+  =
+  map_seq2_len f1 (fst s1) (fst s2);
+  map_seq2_len f2 (snd s1) (snd s2);
+  let x1 = map_seq2 f1 (fst s1) (fst s2) in
+  let x2 = map_seq2 f2 (snd s1) (snd s2) in
+  x1, x2
+
+let op (#a: Type) (#n: nat)
+  (arr1 arr2: array a #n)
+  : array a #n
+  = match arr1, arr2 with
+  | None, f
+  | f, None -> f
+  | Some s1, Some s2 -> Some (op' s1 s2)
+
+let pcm_array' (#a: Type) (#n: nat): pcm' (array a #n) = {
+  composable = composable;
+  op = op;
+  one = None;
+}
+
+let lem_commutative (#a: Type) (#n: nat)
+  (arr1: array a #n)
+  (arr2: array a #n{composable arr1 arr2})
+  : Lemma (op arr1 arr2 == op arr2 arr1)
+  = match arr1, arr2 with
+  | None, _
+  | _, None -> ()
+  | Some s1, Some s2 ->
+      map_seq2_comm f1 (fst s1) (fst s2);
+      map_seq2_comm f2 (snd s1) (snd s2)
+
+let lem_assoc_l_eq (#a: Type) (#n: nat)
+  (arr1 arr2 arr3: array a #n)
+  : Lemma
+  (requires
+    Some? arr1 /\
+    Some? arr2 /\
+    Some? arr3 /\
+    composable arr1 arr2 /\
+    composable arr2 arr3 /\
+    composable (op arr1 arr2) arr3 /\
+    composable arr1 (op arr2 arr3))
+  (ensures
+    op arr1 (op arr2 arr3) == op (op arr1 arr2) arr3)
+  =
+  let s1 = Some?.v arr1 in
+  let s2 = Some?.v arr2 in
+  let s3 = Some?.v arr3 in
+  map_seq2_assoc f1 (fst s1) (fst s2) (fst s3);
+  map_seq2_assoc f2 (snd s1) (snd s2) (snd s3)
+
+let lem_assoc_l_aux1 (#a: Type) (#n: nat)
+  (s1 s2 s3 s23: content a #n)
+  (i: nat)
+  : Lemma
+  (requires
+    i < n /\
+    composable' s2 s3 /\
+    s23 == op' s2 s3 /\
+    comp_prop
+      (index (fst s2) i) (index (fst s3) i)
+      (index (snd s2) i) (index (snd s3) i) /\
+    comp_prop
+      (index (fst s1) i) (index (fst s23) i)
+      (index (snd s1) i) (index (snd s23) i)
+  )
+  (ensures
+    // TODO: duplicata
+    i < n /\
+    comp_prop
+      (index (fst s1) i) (index (fst s2) i)
+      (index (snd s1) i) (index (snd s2) i))
+  =
+  assert (fst s23 == map_seq2 f1 (fst s2) (fst s3));
+  assert (snd s23 == map_seq2 f2 (snd s2) (snd s3));
+  Classical.forall_intro (map_seq2_index f1 (fst s2) (fst s3));
+  Classical.forall_intro (map_seq2_index f2 (snd s2) (snd s3));
+  ()
+
+let lem_assoc_l_aux2 (#a: Type) (#n: nat)
+  (s1 s2 s3 s23 s12: content a #n)
+  (i: nat)
+  : Lemma
+  (requires
+    i < n /\
+    composable' s2 s3 /\
+    s23 == op' s2 s3 /\
+    composable' s1 s2 /\
+    s12 == op' s1 s2 /\
+    comp_prop
+      (index (fst s2) i) (index (fst s3) i)
+      (index (snd s2) i) (index (snd s3) i) /\
+    comp_prop
+      (index (fst s1) i) (index (fst s23) i)
+      (index (snd s1) i) (index (snd s23) i)
+  )
+  (ensures
+    //TODO: duplicata
+    i < n /\
+    comp_prop
+      (index (fst s12) i) (index (fst s3) i)
+      (index (snd s12) i) (index (snd s3) i)
+  )
+  =
+  assert (fst s12 == map_seq2 f1 (fst s1) (fst s2));
+  assert (snd s12 == map_seq2 f2 (snd s1) (snd s2));
+  assert (fst s23 == map_seq2 f1 (fst s2) (fst s3));
+  assert (snd s23 == map_seq2 f2 (snd s2) (snd s3));
+  Classical.forall_intro (map_seq2_index f1 (fst s1) (fst s2));
+  Classical.forall_intro (map_seq2_index f2 (snd s1) (snd s2));
+  Classical.forall_intro (map_seq2_index f1 (fst s2) (fst s3));
+  Classical.forall_intro (map_seq2_index f2 (snd s2) (snd s3))
+
+let lem_assoc_l_aux3 (#a: Type) (#n: nat)
+  (arr1 arr2 arr3: array a #n)
+  : Lemma
+  (requires
+    Some? arr1 /\ Some? arr2 /\ Some? arr3 /\
+    composable arr2 arr3 /\
+    composable arr1 (op arr2 arr3)
+  )
+  (ensures
+    composable arr1 arr2 /\
+    composable (op arr1 arr2) arr3
+  )
+  =
+  let s1 = Some?.v arr1 in
+  let s2 = Some?.v arr2 in
+  let s3 = Some?.v arr3 in
+  let arr23 = op arr2 arr3 in
+  assert (Some? arr23);
+  let s23 = Some?.v arr23 in
+  map_seq2_len f1 (fst s2) (fst s3);
+  map_seq2_len f2 (snd s2) (snd s3);
+  Classical.forall_intro (
+    Classical.move_requires (
+      lem_assoc_l_aux1 #a #n s1 s2 s3 s23
+    )
+  );
+  let arr12 = op arr1 arr2 in
+  assert (Some? arr12);
+  let s12 = Some?.v arr12 in
+  map_seq2_len f1 (fst s1) (fst s2);
+  map_seq2_len f2 (snd s1) (snd s2);
+  Classical.forall_intro (
+    Classical.move_requires (
+      lem_assoc_l_aux2 s1 s2 s3 s23 s12
+    )
+  )
+
+let lem_assoc (#a: Type) (#n: nat)
+  (arr1 arr2 arr3: array a #n)
+  : Lemma
+  (requires
+    composable arr2 arr3 /\
+    composable arr1 (op arr2 arr3)
+  )
+  (ensures
+    composable arr1 arr2 /\
+    composable (op arr1 arr2) arr3 /\
+    op arr1 (op arr2 arr3) == op (op arr1 arr2) arr3
+  )
+  =
+  if None? arr1 then () else
+  if None? arr2 then () else
+  if None? arr3 then () else begin
+  lem_assoc_l_aux3 arr1 arr2 arr3;
+  lem_assoc_l_eq arr1 arr2 arr3;
+  ()
+  end
+
+let lem_assoc_l (#a: Type) (#n: nat)
+  (arr1 arr2: array a #n) (arr3: array a #n{
+    composable arr2 arr3 /\ composable arr1 (op arr2 arr3)
+  })
+  : Lemma (
+    composable arr1 arr2 /\
+    composable (op arr1 arr2) arr3 /\
+    op arr1 (op arr2 arr3) == op (op arr1 arr2) arr3
+  )
+  =
+  lem_assoc arr1 arr2 arr3
+
+let lem_assoc_r (#a: Type) (#n: nat)
+  (arr1 arr2: array a #n) (arr3: array a #n{
+    composable arr1 arr2 /\ composable (op arr1 arr2) arr3
+  })
+  : Lemma (
+    composable arr2 arr3 /\
+    composable arr1 (op arr2 arr3) /\
+    op arr1 (op arr2 arr3) == op (op arr1 arr2) arr3
+  )
+  =
+  lem_commutative arr1 arr2;
+  lem_assoc arr3 arr2 arr1;
+  lem_commutative arr2 arr3;
+  lem_commutative arr1 (op arr2 arr3);
+  lem_commutative arr3 (op arr1 arr2)
+
+let pcm_array (#a: Type) (#n: nat): pcm (array a #n) = {
+  p = pcm_array';
+  comm = lem_commutative;
+  assoc = lem_assoc_l;
+  assoc_r = lem_assoc_r;
+  is_unit = (fun _ -> ());
+  refine = (fun _ -> True);
+}
+
+let array_ref (a: Type u#1) (#n: nat) : Type u#0
+  = Mem.ref (array a #n) pcm_array
+
+let null #a #n = Mem.null #(array a #n) #pcm_array
+let is_null #a #n r = Mem.is_null #(array a #n) #pcm_array r
+
+let perm_ok_elem p : prop = (p.v <=. one == true) /\ True
+
+let perm_ok #n (s: lseq perm n) : prop
+  =
+  forall i. ((index s i).v <=. one == true)
+
+// deprecated
+let apply (#a: Type u#1) (s: seq (a & perm)) (p: perm)
+  : (r:seq (a & perm){length r == length s})
+  =
+  let s', _ = unzip s in
+  unzip_len s;
+  map_seq_len (fun x -> x, p) s';
+  map_seq (fun x -> x, p) s'
+
+// seq (a & perm) or seq a & seq perm?
+// tentative
+//let pts_to_raw_sl_extperm (#a: Type u#1)
+//  (r: array_ref a) (v: content a)
+//  : Mem.slprop u#1
+//  =
+//  let array_with_perm = apply (get_data v) p in
+//  //let new_content = mk_content (get_size v) 0 0 array_with_perm in
+//  let new_content = { v with data = array_with_perm } in
+//  Mem.pts_to r (Some new_content)
+
+// perm is bundled
+let pts_to_raw_sl (#a: Type) (#n: nat)
+  (r: array_ref a #n)
+  (p: lseq perm n)
+  (v: lseq a n)
+  : Mem.slprop
+  = Mem.pts_to r (Some (v, p))
+
+let pts_to_raw (#a: Type) (#n: nat)
+  (r: array_ref a #n)
+  (p: lseq perm n)
+  (v: lseq a n)
+  : vprop
+  //= to_vprop (Mem.pts_to r (Some v))
+  = to_vprop (pts_to_raw_sl r p v)
+
+[@@ __reduce__]
+let pts_to' (#a: Type u#1) (#n: nat)
+  (r: array_ref a)
+  (p: lseq perm n)
+  (v: lseq a n)
+  : vprop
+  =
+  pts_to_raw r p v `star` pure (perm_ok p)
+
+let pts_to_sl #a #n r p v
+  = hp_of (pts_to' #a #n r p v)
+
+let abcd_acbd (a b c d:Mem.slprop)
+  : Lemma (Mem.(((a `star` b) `star` (c `star` d)) `equiv`
+           ((a `star` c) `star` (b `star` d))))
+  = let open Steel.Memory in
+    calc (equiv) {
+    ((a `star` b) `star` (c `star` d));
+      (equiv) { star_associative a b (c `star` d) }
+    ((a `star` (b `star` (c `star` d))));
+      (equiv) { star_associative b c d;
+                star_congruence a (b `star` (c `star` d))
+                                a ((b `star` c) `star` d) }
+    (a `star` ((b `star` c) `star` d));
+      (equiv) { star_commutative  b c;
+                star_congruence (b `star` c) d (c `star` b) d;
+                star_congruence a ((b `star` c) `star` d)
+                                a ((c `star` b) `star` d) }
+    (a `star` ((c `star` b) `star` d));
+      (equiv) { star_associative c b d;
+                star_congruence a ((c `star` b) `star` d)
+                                a (c `star` (b `star` d)) }
+    (a `star` (c `star` (b `star` d)));
+      (equiv) { star_associative a c (b `star` d) }
+    ((a `star` c) `star` (b `star` d));
+   }
+
+let composable_to_fst_eq (#a: Type u#1) (#n: nat)
+  (s1 s2: content a #n)
+  : Lemma
+  (requires composable' s1 s2)
+  (ensures fst s1 == fst s2)
+  =
+  assert (forall (i:nat{i < n}).
+    index (fst s1) i == index (fst s2) i
+  );
+  Seq.lemma_eq_intro (fst s1) (fst s2)
+
+let op_to_fst_eq (#a: Type u#1) (#n: nat)
+  (s1 s2 s3: content a #n)
+  : Lemma
+  (requires
+    composable' s1 s2 /\
+    s3 == op' s1 s2)
+  (ensures fst s1 == fst s3)
+  =
+  Classical.forall_intro (map_seq2_index f1 (fst s1) (fst s2));
+  Seq.lemma_eq_elim (fst s1) (fst s3)
+
+let pts_to_ref_injective (#a: Type u#1) (#n: nat)
+  (r: array_ref a #n)
+  (p0 p1: lseq perm n)
+  (v0 v1: lseq a n)
+  (m:Mem.mem)
+  : Lemma
+    (requires Mem.interp (
+      pts_to_sl r p0 v0 `Mem.star` pts_to_sl r p1 v1) m)
+    (ensures v0 == v1)
+  = let open Steel.Memory in
+    abcd_acbd (hp_of (pts_to_raw r p0 v0))
+              (pure (perm_ok p0))
+              (hp_of (pts_to_raw r p1 v1))
+              (pure (perm_ok p1));
+    Mem.affine_star
+      (hp_of (pts_to_raw r p0 v0) `star` hp_of (pts_to_raw r p1 v1))
+      (pure (perm_ok p0) `star` pure (perm_ok p1)) m;
+    Mem.pts_to_compatible r (Some (v0, p0))
+                            (Some (v1, p1))
+                            m;
+    assert (composable' (v0, p0) (v1, p1));
+    composable_to_fst_eq (v0, p0) (v1, p1)
+
+let pts_to_not_null (#a:Type u#1) (#n: nat)
+                    (r: array_ref a #n)
+                    (p: lseq perm n)
+                    (v: lseq a n)
+                    (m:Mem.mem)
+  : Lemma (requires Mem.interp (pts_to_sl r p v) m)
+          (ensures r =!= null)
+  = Mem.affine_star
+      (hp_of (pts_to_raw r p v))
+      (Mem.pure (perm_ok p)) m;
+    Mem.pts_to_not_null r (Some (v, p)) m
+
+let aux' (#a: Type u#1) (#n: nat)
+  (x y f1 f2 z: array a #n)
+  : Lemma
+  (requires
+    Some? x /\
+    Some? y /\
+    composable x f1 /\
+    op f1 x == z /\
+    composable y f2 /\
+    op f2 y == z
+  )
+  (ensures fst (Some?.v x) == fst (Some?.v y))
+  =
+  assert (Some? z);
+  match (Some? f1, Some? f2) with
+  | false, false -> ()
+  | true, false ->
+    assert (op f2 y == y);
+    assert (y == z);
+    composable_to_fst_eq (Some?.v x) (Some?.v f1);
+    op_to_fst_eq (Some?.v f1) (Some?.v x) (Some?.v z)
+  | false, true ->
+    assert (op f1 x == x);
+    assert (x == z);
+    composable_to_fst_eq (Some?.v y) (Some?.v f2);
+    op_to_fst_eq (Some?.v f2) (Some?.v y) (Some?.v z)
+  | true, true ->
+    composable_to_fst_eq (Some?.v x) (Some?.v f1);
+    composable_to_fst_eq (Some?.v y) (Some?.v f2);
+    op_to_fst_eq (Some?.v f1) (Some?.v x) (Some?.v z);
+    op_to_fst_eq (Some?.v f2) (Some?.v y) (Some?.v z)
+
+let aux (#a: Type u#1) (#n: nat)
+  (r: array_ref a)
+  (p: lseq perm n)
+  (x y: erased (lseq a n))
+  (m:Mem.mem)
+  : Lemma
+  (requires
+    Mem.interp (pts_to_sl r p x) m /\
+    Mem.interp (pts_to_sl r p y) m
+  )
+  (ensures x == y)
+  =
+  let c1 = Some (reveal x, p) in
+  let c2 = Some (reveal y, p) in
+  Mem.pts_to_join r c1 c2 m;
+  assert (joinable pcm_array c1 c2);
+  assert (exists z.
+    compatible pcm_array c1 z /\
+    compatible pcm_array c2 z
+  );
+  assert (
+    exists z.
+    (exists (frame: array a).
+      composable c1 frame /\
+      op frame c1 == z) /\
+    (exists (frame: array a).
+      composable c2 frame /\
+      op frame c2 == z)
+  );
+  assert (
+    exists (z f1 f2: array a).
+      composable c1 f1 /\
+      op f1 c1 == z /\
+      composable c2 f2 /\
+      op f2 c2 == z /\
+      Some? z
+  );
+  Classical.forall_intro_3 (
+    Classical.move_requires_3 (
+        aux' c1 c2
+    )
+  )
+
+// 1) better definition
+// 2) a pts_to wrapper? an unwrapped PCM based on the wrapped one?
+// [selected option] 3) unwrapped PCM from scratch
+let pts_to_witinv_aux (#a:Type) (#n: nat)
+  (r:array_ref a #n) (p: lseq perm n)
+  : Lemma (Mem.is_witness_invariant (pts_to_sl r p))
+  =
+  Classical.forall_intro_3 (
+    fun (x y: lseq a n) ->
+      Classical.move_requires (aux r p x y)
+  )
